Finished the Func feature: domain bounds tests implemented and proved correct

vcfloat/FPLang.v
@@ -76,26 +76,31 @@ Definition default_rel (t: type) : R :=
 Definition default_abs (t: type) : R :=
   / 2 * Raux.bpow Zaux.radix2 (3 - femax t - fprec t).
 
+
+Definition bounds (t: type) : Type :=  (ftype t * bool) * (ftype t * bool).
+Definition interp_bounds {t} (bnds: bounds t) (x: ftype t) : bool :=
+ let '((lo,blo),(hi,bhi)) := bnds in
+ (if blo then BCMP Lt true lo x  else BCMP Gt false lo x) &&
+ (if bhi then BCMP Lt true x hi  else BCMP Gt false x hi).
+
 Fixpoint acc_prop  (args: list type) (result: type)
              (rel abs : N)
-             (precond: function_type (map RR args) Prop)
+             (precond: klist bounds args)
              (rf: function_type (map RR args) R)
              (f: function_type (map ftype' args) (ftype' result)) {struct args} : Prop.
 destruct args as [ | a r].
-Search (N -> R).
-Search (N -> Z).
-exact (precond ->
-                   Binary.is_finite _ _ f = true /\ 
+exact (        Binary.is_finite _ _ f = true /\ 
                    exists delta epsilon,
                   (Rabs delta <= IZR (Z.of_N rel) * default_rel result 
                       /\ Rabs epsilon <= IZR (Z.of_N abs) * default_abs result /\
                    FT2R f = rf * (1+delta) + epsilon)%R).
-exact (forall z: ftype a, Binary.is_finite (fprec a) (femax a) z = true ->
-            acc_prop r result rel abs (precond (FT2R z)) (rf (FT2R z)) (f z)).
+inversion precond as [| ? ? bnds pre]; clear precond; subst.
+exact (forall z: ftype a, interp_bounds bnds z = true -> 
+             acc_prop r result rel abs pre (rf (FT2R z)) (f z)).
 Defined.
 
 Record floatfunc (args: list type) (result: type) 
-     (precond: function_type (map RR args) Prop)
+     (precond: klist bounds args)
      (realfunc: function_type (map RR args) R) := 
  {ff_func: function_type (map ftype' args) (ftype' result);
   ff_rel: N;
@@ -105,7 +110,7 @@ Record floatfunc (args: list type) (result: type)
 
 Record floatfunc_package ty:=
  {ff_args: list type;
-  ff_precond: function_type (map RR ff_args) Prop;
+  ff_precond: klist bounds ff_args;
   ff_realfunc: function_type (map RR ff_args) R;
   ff_ff: floatfunc ff_args ty ff_precond ff_realfunc}.
 
