Test/TestFunc.v
@@ -25,19 +25,25 @@ Definition default_rel (t: type) : R :=
 Definition default_abs (t: type) : R :=
   / 2 * Raux.bpow Zaux.radix2 (3 - femax t - fprec t).
 
-Parameter c_function: forall (args: list type) (res: type) (rel: N) (f: function_type (map RR args) R),
+Parameter c_function: forall (args: list type) (res: type) (bnds: klist bounds args) (rel: N) (f: function_type (map RR args) R),
    {ff: function_type (map ftype' args) (ftype res) 
-   | acc_prop args res rel 1 (always_true args) f ff}.
+   | acc_prop args res rel 1 bnds f ff}.
 
-Ltac floatfunc' args res rel f :=
+Ltac floatfunc' args res bnds rel f :=
  let abs := constr:(1%N) in
- let cf := constr:(c_function args res rel f) in
+ let cf := constr:(c_function args res bnds rel f) in
  let ff1 := constr:(Build_floatfunc args res _ f (proj1_sig cf) rel abs (proj2_sig cf)) in
  exact (Build_floatfunc_package _ _  _ _ ff1).
 
-Definition cosff := ltac:(floatfunc' [Tdouble] Tdouble 3%N Rtrigo_def.cos).
+Definition vacuous_bnds ty : bounds ty := ((B754_infinity (fprec ty) (femax ty) true, false), 
+                              (B754_infinity (fprec ty) (femax ty) false, false)).
+
+Definition silly_bnds : bounds Tdouble :=
+  ((-6, true), (99, false))%F64.
+
+Definition cosff := ltac:(floatfunc' [Tdouble] Tdouble (Kcons (vacuous_bnds Tdouble) Knil) 3%N Rtrigo_def.cos).
 Definition cos := ltac:(apply_func cosff).
-Definition sinff := ltac:(floatfunc' [Tdouble] Tdouble 5%N Rtrigo_def.sin).
+Definition sinff := ltac:(floatfunc' [Tdouble] Tdouble (Kcons silly_bnds Knil) 5%N Rtrigo_def.sin).
 Definition sin := ltac:(apply_func sinff).
 
 Lemma test_reify1: False.
@@ -120,7 +126,7 @@ intros.
 prove_roundoff_bound.
 -
 prove_rndval.
- all: interval.
+all: interval.
 - 
 prove_roundoff_bound2.
  match goal with |- Rabs ?a <= _ => field_simplify a end. (* improves the bound *)
